src/cddl/spec/CDDL.Spec.Misc.fst
@@ -1,0 +1,135 @@
+module CDDL.Spec.Misc
+include CDDL.Spec.Base
+module Cbor = CBOR.Spec.API.Format
+module U8 = FStar.UInt8
+module U64 = FStar.UInt64
+
+// Appendix D
+
+let uint : typ = (fun w -> let x = Cbor.unpack w in Cbor.CInt64? x && Cbor.CInt64?.typ x = Cbor.cbor_major_type_uint64)
+let nint : typ = (fun w -> let x = Cbor.unpack w in Cbor.CInt64? x && Cbor.CInt64?.typ x = Cbor.cbor_major_type_neg_int64)
+let t_int : typ = uint `t_choice` nint
+
+let bstr : typ = (fun w -> let x = Cbor.unpack w in Cbor.CString? x && Cbor.CString?.typ x = Cbor.cbor_major_type_byte_string)
+let bytes = bstr
+let tstr : typ = (fun w -> let x = Cbor.unpack w in Cbor.CString? x && Cbor.CString?.typ x = Cbor.cbor_major_type_text_string)
+let text = tstr
+
+[@@CMacro]
+let simple_value_false : Cbor.simple_value = 20uy
+[@@CMacro]
+let simple_value_true : Cbor.simple_value = 21uy
+[@@CMacro]
+let simple_value_nil : Cbor.simple_value = 22uy
+[@@CMacro]
+let simple_value_undefined : Cbor.simple_value = 23uy
+
+let t_simple_value_literal (s: Cbor.simple_value) : typ =
+  t_literal (Cbor.pack (Cbor.CSimple s))
+
+let t_false : typ = t_simple_value_literal simple_value_false
+let t_true : typ = t_simple_value_literal simple_value_true
+let t_bool : typ = t_choice t_false t_true
+let t_nil : typ = t_simple_value_literal simple_value_nil
+let t_null : typ = t_nil
+let t_undefined : typ = t_simple_value_literal simple_value_undefined
+
+let t_uint_literal (v: U64.t) : typ =
+  t_literal (Cbor.pack (Cbor.CInt64 Cbor.cbor_major_type_uint64 v))
+
+// 2.1 specifies "names that turn into the map key text string"
+
+noextract
+let string64 = (s: Seq.seq U8.t {FStar.UInt.fits (Seq.length s) 64})
+
+let name_as_text_string (s: string64) : typ =
+  t_literal (Cbor.pack (Cbor.CString Cbor.cbor_major_type_text_string s))
+
+// Section 3.6: Tags
+
+(*
+let t_tag (#b: option Cbor.cbor) (tag: U64.t) (t: bounded_typ_gen b) : bounded_typ_gen b = fun w -> let x = Cbor.unpack w in
+  Cbor.CTagged? x &&
+  Cbor.CTagged?.tag x = tag &&
+  t (Cbor.CTagged?.v x)
+
+let rec t_tag_rec
+  (tag: U64.t)
+  (phi: (b: Cbor.raw_data_item) -> (bounded_typ b -> bounded_typ b))
+  (x: Cbor.raw_data_item)
+: GTot bool
+  (decreases x)
+= Cbor.Tagged? x &&
+  Cbor.Tagged?.tag x = tag &&
+  phi x (t_tag_rec tag phi) (Cbor.Tagged?.v x)
+*)
+let t_tag (tag: U64.t) (t: typ) : typ = fun w -> let x = Cbor.unpack w in
+  Cbor.CTagged? x &&
+  Cbor.CTagged?.tag x = tag &&
+  t (Cbor.CTagged?.v x)
+
+let spec_tag
+  (tag: U64.t)
+  (#t: typ)
+  (#target: Type)
+  (p: spec t target)
+: Tot (spec (t_tag tag t) target)
+= {
+  serializable = p.serializable;
+  parser = (function w -> let Cbor.CTagged _ v = Cbor.unpack w in p.parser v);
+  serializer = (fun x -> Cbor.pack (Cbor.CTagged tag (p.serializer x)));
+}
+
+// Section 3.8.1: Control .size
+
+let str_size (ty: Cbor.major_type_byte_string_or_text_string) (sz: nat) : typ = fun w -> let x = Cbor.unpack w in
+  Cbor.CString? x &&
+  Cbor.CString?.typ x = ty &&
+  Seq.length (Cbor.CString?.v x) = sz
+
+let uint_size (sz: nat) : typ = fun w -> let x = Cbor.unpack w in
+  Cbor.CInt64? x &&
+  Cbor.CInt64?.typ x = Cbor.cbor_major_type_uint64 &&
+  U64.v (Cbor.CInt64?.v x) < pow2 sz
+
+// Section 3.8.4: Control .cbor
+
+let bstr_cbor
+  (ty: typ) // TODO: enable recursion for this construct? If so, we need to replace << with some serialization size
+: typ = fun w -> let x = Cbor.unpack w in
+  Cbor.CString? x &&
+  Cbor.CString?.typ x = Cbor.cbor_major_type_byte_string &&
+  begin match Cbor.cbor_parse (Cbor.CString?.v x) with
+  | None -> false
+  | Some (y, consumed) -> consumed = Seq.length (Cbor.CString?.v x) && ty y
+  end
+
+let bstr_cbor_det
+  (ty: typ) // TODO: enable recursion for this construct? If so, we need to replace << with some serialization size
+: typ = fun w -> let x = Cbor.unpack w in
+  Cbor.CString? x &&
+  Cbor.CString?.typ x = Cbor.cbor_major_type_byte_string &&
+  begin match Cbor.cbor_det_parse (Cbor.CString?.v x) with
+  | None -> false
+  | Some (y, consumed) -> consumed = Seq.length (Cbor.CString?.v x) && ty y
+  end
+
+let parser_spec_bool (p: bool -> prop { forall x . p x }) : parser_spec t_bool bool p =
+  (fun x -> let Cbor.CSimple v = Cbor.unpack x in
+    v = simple_value_true
+  )
+
+let serializer_spec_bool (p: bool -> prop { forall x . p x }) : serializer_spec (parser_spec_bool p) =
+  (fun x -> Cbor.pack (Cbor.CSimple (if x then simple_value_true else simple_value_false)))
+
+let parser_spec_bstr (p: string64 -> prop { forall x . p x }) : parser_spec bstr string64 p =
+  (fun x -> let Cbor.CString _ v = Cbor.unpack x in v)
+
+let serializer_spec_bstr (p: string64 -> prop { forall x . p x }) : serializer_spec (parser_spec_bstr p) =
+  (fun x -> Cbor.pack (Cbor.CString Cbor.cbor_major_type_byte_string x))
+
+let parser_spec_tstr (p: string64 -> prop { forall x . p x }) : parser_spec tstr string64 p =
+  (fun x -> let Cbor.CString _ v = Cbor.unpack x in v)
+
+let serializer_spec_tstr (p: string64 -> prop { forall x . p x }) : serializer_spec (parser_spec_tstr p) =
+  (fun x -> Cbor.pack (Cbor.CString Cbor.cbor_major_type_text_string x))
